% SECTION ====================================================================================
\section{Mathematical background}
% ============================================================================================
\subsection{General}
\subsubsection{Matrix inverse}
$\begin{bmatrix}a_{11}&a_{12}\\a_{21}&a_{22}\end{bmatrix}^{-1}=
\frac{1}{a_{11}a_{22}-a_{12}a_{21}}\begin{bmatrix}a_{22}&-a_{12}\\-a_{21}&a_{11}\end{bmatrix}$
\subsubsection{Hermitian matrix}
$\begin{bmatrix}a_{11}&a_{12}\\a_{21}&a_{22}\end{bmatrix}^{H}=
\begin{bmatrix}a_{11}^*&a_{21}^*\\a_{12}^*&a_{22}^*\end{bmatrix}$

\subsubsection{Quadratic equation}
$ax^2+bx+c=0\pfeil x_{1/2}=\frac{-b\pm\sqrt{b^2-4ac}}{2a}$\\
$x^2 + px + q=0 \pfeil x_{1/2}=-\frac{p}{2} \pm \sqrt{\frac{p^2}{4}-q} $\\

\subsubsection{Euklidian Norm}
$||\vec{v}||_2=\sqrt{v_1^2 + v_2^2 + ... + v_N} = \sqrt{\sum_{i=1}^{N}|v_i|^2}$
\subsubsection{Frobenius Norm}
$||\ma{V}||_F=\sqrt{|v_{1,1}|^2 + |v_{1,2}|^2+... + |v_{N,M}|^2} =\sqrt{\sum_{i=1}^{N} \sum_{j=1}^{M}|v_{i,j}|^2}$
\subsubsection{Taylor series}
$T f(x, a)  = \sum_{n=0}^\infty  \frac{f^{(n)}(a)}{n!} (x-a)^n = f(a) + f'(a) (x-a) + \frac{f''(a)}{2}(x-a)^2 + \frac{f'''(a)}{6} (x-a)^3 + \ldots$
\subsubsection{Fourier series}
$f(t)=\frac{a_{0}}{2}+\sum_{k=1}^{\infty}\left(a_{k}\cos\left(kt\right)+b_{k}\sin\left(kt\right)\right)$\\
$a_{k}=c_{k}+c_{-k}\quad\text{f端r }k\geq0$\\
$b_{k}=\mathrm{i}\left(c_{k}-c_{-k}\right)\quad\text{f端r }k\geq1$\\
or as an alternative:\\
$a_{k} = \frac{1}{\pi}\int_{-\pi}^{\pi}f(t)\cdot\cos\left(kt\right)\mathrm dt\quad\text{f端r }k\geq0$\\
$b_{k} = \frac{1}{\pi}\int_{-\pi}^{\pi}f(t)\cdot\sin\left(kt\right)\mathrm dt\quad\text{f端r }k\geq1$
